h2k: succeeded to reify one of the rules defined in the case study; (almost) compiled it to a Kami rule.

syn/HemiolaDeep.v
@@ -4,103 +4,150 @@ Require Import Hemiola.RqRsLang.
         
 Set Implicit Arguments.
 
+Definition TODO := cheat.
+
 Import MonadNotations.
 
-(* {| ost_ty := [nat:Type; bool:Type; MESI:Type; DirT:Type]%vector |}. *)
+(** Configuration class *)
 
-(* Inductive HTypes {t} (var: Type -> t): forall {sz}, Vector.t Type sz -> Type := *)
-(* | HTyNil: HTypes var (Vector.nil _) *)
-(* | HTyCons: *)
-(*     forall {sz} {tys: Vector.t Type sz}, *)
-(*       HTypes var tys -> *)
-(*       forall {ty}, *)
-(*         HType var ty -> *)
-(*         HTypes var (ty :: tys). *)
-
-(* Record HOStateIfc (oifc: OStateIfc) := *)
-(*   { host_ty: HTypes (@ost_ty oifc); *)
-(*     host_init: *)
-(*   }. *)
+Class hconfig :=
+  { hcfg_oidx_sz: nat;
+    hcfg_oidx_deg: nat;
+    hcfg_midx_sz: nat;
+    hcfg_midx_deg: nat;
+    hcfg_msg_id_sz: nat;
+    hcfg_msg_id_deg: nat;
+    hcfg_value_sz: nat }.
 
 Section Reify.
   Context `{DecValue} `{oifc: OStateIfc}.
+  Context `{hconfig}.
 
   (** Reified syntax *)
-  
-  (* -- basis *)
-  
-  Inductive HValue: Type -> Type :=
-  | HConst: forall {ty} (c: ty), HValue ty
-  | HOstVal: forall idx, HValue (Vector.nth (@ost_ty oifc) idx).
-
-  (* -- for precondition *)
-  
-  Inductive HOPrecP: Type :=
-  | HAnd: HOPrecP -> HOPrecP -> HOPrecP
-  | HOr: HOPrecP -> HOPrecP -> HOPrecP
-  | HBoolT: HValue bool -> HOPrecP
-  | HBoolF: HValue bool -> HOPrecP
-  | HNatEq (sz: nat): HValue nat -> HValue nat -> HOPrecP
-  | HNatNe (sz: nat): HValue nat -> HValue nat -> HOPrecP
-  | HNatLt (sz: nat): HValue nat -> HValue nat -> HOPrecP
-  | HNatLe (sz: nat): HValue nat -> HValue nat -> HOPrecP
-  | HNatGt (sz: nat): HValue nat -> HValue nat -> HOPrecP
-  | HNatGe (sz: nat): HValue nat -> HValue nat -> HOPrecP.
-
-  Inductive HOPrecR: Type :=
-  | HRqAccepting: HOPrecR
-  | HRsAccepting: HOPrecR
-  | HUpLockFree: HOPrecR
-  | HDownLockFree: HOPrecR
-  | HUpLockMsgId (mty: bool) (mid: IdxT): HOPrecR
-  | HUpLockMsg: HOPrecR
-  | HUpLockIdxBack: HOPrecR
-  | HUpLockBackNone: HOPrecR
-  | HDownLockMsgId (mty: bool) (mid: IdxT): HOPrecR
-  | HDownLockMsg: HOPrecR
-  | HDownLockIdxBack: HOPrecR
-  | HMsgIdFrom (msgId: IdxT): HOPrecR.
-
-  Inductive HMsgFrom: Type :=
-  | HMsgFromParent: HMsgFrom
-  | HMsgFromChild (cidx: IdxT): HMsgFrom.
-
-  Inductive HOPrec: Type :=
-  | HOPrecAnd: HOPrec -> HOPrec -> HOPrec
-  | HOPrecRqRs: HOPrecR -> HOPrec
-  | HOPrecProp: HOPrecP -> HOPrec.
-
-  (* -- for transition *)
 
   Inductive htype :=
-  | HIdx | HMsg.
+  | HBool
+  | HIdx (width: nat)
+  | HNat (width: nat)
+  | HValue
+  | HMsg
+  | HPair: htype -> htype -> htype.
 
-  Definition htypeDenote (ht: htype): Type :=
+  Definition HIdxO := HIdx hcfg_oidx_sz.
+  Definition HIdxQ := HIdx hcfg_midx_sz.
+  Definition HIdxM := HIdx hcfg_msg_id_sz.
+
+  Fixpoint htypeDenote (ht: htype): Type :=
     match ht with
-    | HIdx => IdxT
+    | HBool => bool
+    | HIdx _ => IdxT
+    | HNat _ => nat
+    | HValue => t_type
     | HMsg => Msg
+    | HPair ht1 ht2 => htypeDenote ht1 * htypeDenote ht2
     end.
 
-  Section Transition.
+  Section Phoas.
     Variable var: htype -> Type.
     
-    Inductive HBindValue: htype -> Type :=
-    | HGetFirstMsg: HBindValue HMsg
-    | HGetUpLockMsg: HBindValue HMsg
-    | HGetDownLockMsg: HBindValue HMsg
-    | HGetUpLockIdxBack: HBindValue HIdx
-    | HGetDownLockIdxBack: HBindValue HIdx.
+    (* -- constants and expressions *)
 
-    Inductive HOState := .
-    Inductive HORq := .
-    Inductive HMsgsOut := .
+    Inductive hconst: htype -> Type :=
+    | HConstBool: forall b: bool, hconst HBool
+    | HConstNat: forall w (n: nat), hconst (HNat w)
+    | HConstIdx: forall w (deg: nat) (i: IdxT), hconst (HIdx w).
+
+    Inductive hexp: htype -> Type :=
+    | HConst: forall ht (c: hconst ht), hexp ht
+    | HVar: forall ht, var ht -> hexp ht
+    | HMsgB: hexp HIdxM -> hexp HBool -> hexp HValue -> hexp HMsg
+    | HIdm: hexp HIdxQ -> hexp HMsg -> hexp (HPair HIdxQ HMsg)
+    | HOstVal: forall i ht,
+        Vector.nth (@ost_ty oifc) i = htypeDenote ht -> hexp ht.
+
+    (* -- precondition *)
+    
+    Inductive HOPrecP: Type :=
+    | HAnd: HOPrecP -> HOPrecP -> HOPrecP
+    | HOr: HOPrecP -> HOPrecP -> HOPrecP
+    | HBoolT: hexp HBool -> HOPrecP
+    | HBoolF: hexp HBool -> HOPrecP
+    | HEq: forall {ht}, hexp ht -> hexp ht -> HOPrecP
+    | HNe: forall {ht}, hexp ht -> hexp ht -> HOPrecP
+    | HNatLt: forall {w}, hexp (HNat w) -> hexp (HNat w) -> HOPrecP
+    | HNatLe: forall {w}, hexp (HNat w) -> hexp (HNat w) -> HOPrecP
+    | HNatGt: forall {w}, hexp (HNat w) -> hexp (HNat w) -> HOPrecP
+    | HNatGe: forall {w}, hexp (HNat w) -> hexp (HNat w) -> HOPrecP.
+
+    Inductive HOPrecR: Type :=
+    | HRqAccepting: HOPrecR
+    | HRsAccepting: HOPrecR
+    | HUpLockFree: HOPrecR
+    | HDownLockFree: HOPrecR
+    | HUpLockMsgId (mty: bool) (mid: IdxT): HOPrecR
+    | HUpLockMsg: HOPrecR
+    | HUpLockIdxBack: HOPrecR
+    | HUpLockBackNone: HOPrecR
+    | HDownLockMsgId (mty: bool) (mid: IdxT): HOPrecR
+    | HDownLockMsg: HOPrecR
+    | HDownLockIdxBack: HOPrecR
+    | HMsgIdFrom (msgId: IdxT): HOPrecR.
+
+    Inductive HMsgFrom: Type :=
+    | HMsgFromParent: HMsgFrom
+    | HMsgFromChild (cidx: IdxT): HMsgFrom.
+
+    Inductive HOPrecT: Type :=
+    | HOPrecAnd: HOPrecT -> HOPrecT -> HOPrecT
+    | HOPrecRqRs: HOPrecR -> HOPrecT
+    | HOPrecProp: HOPrecP -> HOPrecT.
+
+    (* -- transition *)
+
+    Inductive hbval: htype -> Type :=
+    | HGetFirstMsg: hbval HMsg
+    | HGetUpLockMsg: hbval HMsg
+    | HGetDownLockMsg: hbval HMsg
+    | HGetUpLockIdxBack: hbval HIdxQ
+    | HGetDownLockIdxBack: hbval HIdxQ.
+
+    Inductive HOState :=
+    | HOStateI: HOState.
+      
+    Inductive HORq :=
+    | HORqI: HORq
+    | HUpdUpLock: hexp HMsg ->
+                  hexp HIdxQ (* response-from *) ->
+                  hexp HIdxQ (* response-back-to *) -> HORq
+    | HRelUpLock: HORq
+    | HUpdDownLock: hexp HMsg ->
+                    list (hexp HIdxQ) (* responses-from *) ->
+                    hexp HIdxQ (* response-back-to *) -> HORq
+    | HRelDownLock.
+    
+    Inductive HMsgsOut :=
+    | HMsgsOutI: list (hexp (HPair HIdxQ HMsg)) -> HMsgsOut.
 
     Inductive HMonadT: Type :=
-    | HBind: forall {ht} (bv: HBindValue ht) (cont: var ht -> HMonadT), HMonadT
+    | HBind: forall {ht} (bv: hbval ht) (cont: var ht -> HMonadT), HMonadT
     | HRet: HOState -> HORq -> HMsgsOut -> HMonadT.
 
-  End Transition.
+  End Phoas.
 
+  Arguments HConst {var}.
+  Arguments HVar {var}.
+  Arguments HMsgB {var}.
+  Arguments HIdm {var}.
+  Arguments HOstVal {var}.
+  Arguments HORqI {var}.
+  Arguments HUpdUpLock {var}.
+  Arguments HRelUpLock {var}.
+  Arguments HUpdDownLock {var}.
+  Arguments HRelDownLock {var}.
+  Arguments HMsgsOutI {var}.
+  Arguments HOPrecRqRs {var}.
+
+  Definition HOPrec := forall var, HOPrecT var.
   Definition HMonad := forall var, HMonadT var.
 
   Inductive HStateMTrs: Type :=
@@ -111,27 +158,43 @@ Section Reify.
 
   (** Interpretation *)
   
-  Section Interp.
+  Section WithPreState.
     Variables (ost: OState) (orq: ORq Msg) (mins: list (Id Msg)).
 
-    Definition interpValue {ty} (hv: HValue ty): ty :=
-      match hv with
-      | HConst c => c
-      | HOstVal idx => (ost#[idx])%hvec
+    Definition interpConst {ht} (c: hconst ht): htypeDenote ht :=
+      match c with
+      | HConstBool b => b
+      | HConstNat _ n => n
+      | HConstIdx _ _ i => i
       end.
 
-    Fixpoint interpOPrecP (p: HOPrecP): Prop :=
+    Fixpoint interpExp {ht} (e: hexp htypeDenote ht): htypeDenote ht :=
+      match e with
+      | HConst _ c => interpConst c
+      | HVar _ hv => hv
+      | HMsgB mid mty mval =>
+        {| msg_id := interpExp mid;
+           msg_type := interpExp mty;
+           msg_value := interpExp mval |}
+      | HIdm midx msg => (interpExp midx, interpExp msg)
+      | HOstVal i ht Heq =>
+        match Heq with
+        | eq_refl => (ost#[i])%hvec
+        end
+      end.
+
+    Fixpoint interpOPrecP (p: HOPrecP htypeDenote): Prop :=
       match p with
       | HAnd p1 p2 => interpOPrecP p1 /\ interpOPrecP p2
       | HOr p1 p2 => interpOPrecP p1 \/ interpOPrecP p2
-      | HBoolT b => interpValue b = true
-      | HBoolF b => interpValue b = false
-      | HNatEq _ v1 v2 => interpValue v1 = interpValue v2
-      | HNatNe _ v1 v2 => interpValue v1 <> interpValue v2
-      | HNatLt _ v1 v2 => interpValue v1 < interpValue v2
-      | HNatLe _ v1 v2 => interpValue v1 <= interpValue v2
-      | HNatGt _ v1 v2 => interpValue v1 > interpValue v2
-      | HNatGe _ v1 v2 => interpValue v1 >= interpValue v2
+      | HBoolT b => interpExp b = true
+      | HBoolF b => interpExp b = false
+      | HEq v1 v2 => interpExp v1 = interpExp v2
+      | HNe v1 v2 => interpExp v1 <> interpExp v2
+      | HNatLt v1 v2 => interpExp v1 < interpExp v2
+      | HNatLe v1 v2 => interpExp v1 <= interpExp v2
+      | HNatGt v1 v2 => interpExp v1 > interpExp v2
+      | HNatGe v1 v2 => interpExp v1 >= interpExp v2
       end.
 
     Definition interpOPrecR (p: HOPrecR): Prop :=
@@ -156,7 +219,7 @@ Section Reify.
       | HMsgFromChild cidx => MsgsFrom [cidx] ost orq mins
       end.
 
-    Definition interpBindValue {bt} (bv: HBindValue bt): option (htypeDenote bt) :=
+    Definition interpBindValue {bt} (bv: hbval bt): option (htypeDenote bt) :=
       match bv with
       | HGetFirstMsg => getFirstMsg mins
       | HGetUpLockMsg => getUpLockMsg orq
@@ -165,9 +228,30 @@ Section Reify.
       | HGetDownLockIdxBack => getDownLockIdxBack orq
       end.
 
-  End Interp.
+    Definition interpOState (host: HOState): OState :=
+      match host with
+      | HOStateI => ost
+      end.
 
-  Fixpoint interpOPrec (p: HOPrec): OPrec :=
+    Definition interpORq (horq: HORq htypeDenote): ORq Msg :=
+      match horq with
+      | HORqI => orq
+      | HUpdUpLock rq rsf rsb =>
+        addRq orq upRq (interpExp rq) [interpExp rsf] (interpExp rsb)
+      | HRelUpLock => removeRq orq upRq
+      | HUpdDownLock rq rssf rsb =>
+        addRq orq downRq (interpExp rq) (List.map interpExp rssf) (interpExp rsb)
+      | HRelDownLock => removeRq orq downRq
+      end.
+
+    Definition interpMsgOuts (houts: HMsgsOut htypeDenote): list (Id Msg) :=
+      match houts with
+      | HMsgsOutI outs => List.map interpExp outs
+      end.
+    
+  End WithPreState.
+
+  Fixpoint interpOPrec (p: HOPrecT htypeDenote): OPrec :=
     match p with
     | HOPrecAnd p1 p2 => interpOPrec p1 /\oprec interpOPrec p2
     | HOPrecRqRs rp => fun ost orq mins => interpOPrecR ost orq mins rp
@@ -179,7 +263,10 @@ Section Reify.
     | HBind bv cont =>
       (msg <-- interpBindValue (orq stm) (msgs stm) bv;
       interpMonad (cont msg) stm)
-    | HRet _ _ _ _ => None
+    | HRet host horq houts =>
+      Some {| ost := interpOState (ost stm) host;
+              orq := interpORq (ost stm) (orq stm) horq;
+              msgs := interpMsgOuts (ost stm) houts |}
     end.
 
   Definition interpMTrs (trs: HStateMTrs): StateMTrs :=
@@ -195,7 +282,7 @@ Section Reify.
 End Reify.
 
 Section HemiolaDeep.
-  Context `{DecValue} `{OStateIfc}.
+  Context `{DecValue} `{OStateIfc} `{hconfig}.
 
   Record HRule (sr: Rule) :=
     { hrule_msg_from: HMsgFrom;
@@ -203,7 +290,7 @@ Section HemiolaDeep.
       hrule_precond_ok:
         forall ost orq mins,
           (interpMsgFrom ost orq mins hrule_msg_from /\
-           interpOPrec hrule_precond ost orq mins)
+           interpOPrec (hrule_precond htypeDenote) ost orq mins)
           <-> rule_precond sr ost orq mins;
       hrule_trs: HOTrs;
       hrule_trs_ok:
@@ -226,4 +313,114 @@ Section HemiolaDeep.
 End HemiolaDeep.
 
 Arguments hvec_ith: simpl never.
+
+
+
+(** * Temporary Testing Section *)
+Require Import Hemiola.Ex.TopoTemplate Hemiola.Ex.RuleTemplate.
+Require Import Hemiola.Ex.Mesi.Mesi.
+
+Require Import FunctionalExtensionality.
+
+Lemma abcd: forall A B C D, (A <-> B) -> (C <-> D) -> (A /\ C <-> B /\ D).
+Proof. firstorder. Qed.
+
+Section Tests.
+
+  Lemma TrsMTrs_ext:
+    forall `{DecValue} `{OStateIfc} (trs1 trs2: StateMTrs),
+      (forall stm, trs1 stm = trs2 stm) ->
+      forall ost orq mins,
+        TrsMTrs trs1 ost orq mins = TrsMTrs trs2 ost orq mins.
+  Proof.
+    cbv [TrsMTrs]; intros.
+    rewrite H1; reflexivity.
+  Qed.
+
+  Variable oidx: IdxT.
+
+  Instance mesiHConfig: hconfig :=
+    {| hcfg_oidx_sz := 8;
+       hcfg_oidx_deg := 4;
+       hcfg_midx_sz := 10;
+       hcfg_midx_deg := 16;
+       hcfg_msg_id_sz := 5;
+       hcfg_msg_id_deg := 4;
+       hcfg_value_sz := 32 |}.
+
+  Existing Instance Mesi.ImplOStateIfc.
+
+  Definition hl1GetSImm: HRule (l1GetSImm (l1ExtOf oidx)).
+  Proof.
+    refine {| hrule_msg_from := _ |}.
+
+    - intros.
+      repeat autounfold with MesiRules.
+      cbv [immDownRule].
+      cbv [rule_precond].
+
+      apply abcd.
+
+      + cbv [interpMsgFrom].
+        instantiate (1:= HMsgFromChild _).
+        apply iff_refl.
+
+      + instantiate (1:= fun var => HOPrecAnd (var:= var) _ _); simpl; apply abcd.
+        all: repeat
+               match goal with
+               | |- _ <-> (_ /\oprec _) _ _ _ =>
+                 instantiate (1:= HOPrecAnd _ _); simpl; apply abcd
+               end.
+
+        1-4: instantiate (1:= HOPrecRqRs _ _); simpl.
+        1-4: first [instantiate (1:= HRqAccepting); apply iff_refl; fail
+                   |instantiate (1:= HRsAccepting); apply iff_refl; fail
+                   |instantiate (1:= HUpLockFree); apply iff_refl; fail
+                   |instantiate (1:= HDownLockFree); apply iff_refl; fail
+                   |instantiate (1:= HUpLockMsgId _ _); apply iff_refl; fail
+                   |instantiate (1:= HUpLockMsg); apply iff_refl; fail
+                   |instantiate (1:= HUpLockIdxBack); apply iff_refl; fail
+                   |instantiate (1:= HUpLockBackNone); apply iff_refl; fail
+                   |instantiate (1:= HDownLockMsgId _ _); apply iff_refl; fail
+                   |instantiate (1:= HDownLockMsg); apply iff_refl; fail
+                   |instantiate (1:= HDownLockIdxBack); apply iff_refl; fail
+                   |instantiate (1:= HMsgIdFrom _); apply iff_refl; fail].
+
+        instantiate (1:= HOPrecProp _); simpl.
+        instantiate (1:= HNatLe (w:= 2) _ _); simpl.
+        instantiate (2:= HConst _ (HConstNat _ Mesi.mesiS)); simpl.
+        instantiate (1:= HOstVal _ status (HNat _) eq_refl).
+        apply iff_refl.
+
+    - intros.
+      repeat autounfold with MesiRules.
+      cbv [immDownRule].
+      cbv [rule_trs].
+
+      instantiate (1:= HTrsMTrs (HMTrs _)); simpl.
+      apply TrsMTrs_ext; intros.
+      instantiate (1:= fun var => HBind (var:= var) _ _); simpl.
+      instantiate (3:= HGetFirstMsg); simpl.
+      instantiate (1:= fun msg => HRet _ _ _).
+      simpl; repeat f_equal.
+      apply functional_extensionality; intros msg.
+      repeat f_equal.
+      { instantiate (1:= HOStateI); reflexivity. }
+      { instantiate (1:= HORqI _); reflexivity. }
+      { instantiate (1:= HMsgsOutI [_]).
+        simpl; repeat f_equal.
+        instantiate (1:= HIdm _ _).
+        simpl; repeat f_equal.
+        { instantiate (1:= HConst _ (HConstIdx _ hcfg_midx_deg _)); reflexivity. }
+        { cbv [rsMsg miv_id miv_value].
+          instantiate (1:= HMsgB _ _ _).
+          simpl; f_equal.
+          { instantiate (1:= HConst _ (HConstIdx _ hcfg_msg_id_deg _)); reflexivity. }
+          { instantiate (1:= HConst _ (HConstBool _)); reflexivity. }
+          { instantiate (1:= HOstVal _ val HValue eq_refl); reflexivity. }
+        }
+      }
+  Defined.
+
+End Tests.
 
